coq/LLVMGen/Correctness_NExpr.v
@@ -1,9 +1,6 @@
 Require Import Helix.LLVMGen.Correctness_Prelude.
+Require Import Helix.LLVMGen.Freshness.
 Require Import Helix.LLVMGen.Correctness_Invariants.
-Require Import Helix.LLVMGen.StateInvariant.
-Require Import Helix.LLVMGen.VariableBinding.
-Require Import Helix.LLVMGen.LidBound.
-Require Import Helix.LLVMGen.IdLemmas.
 
 (* Import ProofNotations. *)
 Import ListNotations.
@@ -94,210 +91,6 @@ Section NExpr.
 
   Import ProofMode.
 
-  Lemma genNExpr_local_count :
-    forall nexp s1 s2 e c,
-      genNExpr nexp s1 ≡ inr (s2, (e, c)) ->
-      (local_count s2 >= local_count s1)%nat.
-  Proof.
-    induction nexp;
-      intros s1 s2 e c GEN;
-      cbn in GEN; simp;
-        repeat
-          match goal with
-          | H: ErrorWithState.option2errS _ (nth_error (Γ ?s1) ?n) ?s1 ≡ inr (?s2, _) |- _ =>
-            destruct (nth_error (Γ s1) n) eqn:FIND; inversion H; subst
-          | H : incLocal ?s1 ≡ inr (?s2, _) |- _ =>
-            apply incLocal_local_count in H
-          | IH : ∀ (s1 s2 : IRState) (e : exp typ) (c : code typ),
-              genNExpr ?n s1 ≡ inr (s2, (e, c)) → local_count s2 ≥ local_count s1,
-      GEN: genNExpr ?n _ ≡ inr _ |- _ =>
-    apply IH in GEN
-    end;
-      try lia.
-  Qed.
-
-  Ltac get_local_count_hyps ::=
-    repeat
-      match goal with
-      | H: incBlockNamed ?n ?s1 ≡ inr (?s2, _) |- _ =>
-        apply incBlockNamed_local_count in H
-      | H: incVoid ?s1 ≡ inr (?s2, _) |- _ =>
-        apply incVoid_local_count in H
-      | H: incLocal ?s1 ≡ inr (?s2, _) |- _ =>
-        apply incLocal_local_count in H
-      | H: genNExpr ?n ?s1 ≡ inr (?s2, _) |- _ =>
-        apply genNExpr_local_count in H
-      end.
-
-  Create HintDb irs_lt.
-  Hint Resolve incLocal_lt : irs_lt.
-  
-  Ltac solve_alist_fresh :=
-    (eapply freshness_pre_alist_fresh; now eauto with irs_lt).
-  
-  Ltac solve_sub_alist :=
-    (reflexivity
-     || (apply sub_alist_add; solve_alist_fresh)
-     || (etransitivity; try eassumption; []; solve_sub_alist)
-    ).
-
-Lemma alist_In_dec :
-  forall {K V} `{RelDec K} `{RelDec v} (id : K) (l : alist K V) (v : V),
-    {alist_In id l v} + {~(alist_In id l v)}.
-Proof.
-Admitted.
-
-Require Import LidBound.
-
-  (* Lemma freshness_chain: forall s1 s2 s3 g1 g2 l1 l2 memV1 memV2 , *)
-  (*     freshness_pre s1 s3 (memV1,(l1,g1)) -> *)
-  (*     freshness_post s1 s2 l1 (memV2,(l2,g2)) -> *)
-  (*     freshness_pre s2 s3 (memV2,(l2,g2)). *)
-  (* Proof. *)
-  (*   intros * PRE POST. *)
-  (*   cbn in *. *)
-  (*   intros * IN. *)
-  (*   destruct (alist_In_dec id l1 v) as [IN' | NIN]. *)
-  (*   - apply PRE in IN'. *)
-
-  (* Admitted. *)
-
-  (** * Freshness
-      We need to reason about the freshness of local variables generated through the IRState monad.
-      To this end, we rely on the following pre and postcondition about local states when reasoning about a given computation c:
-      - freshness_pre s1 s2 : fun l => dom(l) ∩ [s1,s2] = ∅
-        i.e. we ensure that the provided interval over which we will generate variables is indeed fresh
-      - freshness_post s1 s2 li : fun lf => dom(lf) \ dom(li) ⊆ [s1;s2]
-        i.e. after the computation, the new local state has indeed only been extended with variables from the provided interval.
-
-     Let us note FP (resp. FQ) for freshness_pre (resp. freshness_post). We have the following lemmas axiomatizing how these two predicates evolve.
-
-     P1. FP s s l             : if we give ourself an empty freshness window, the precondition is trivially true
-
-     P2. FP s1 s3 l ->
-          s2 << s3 ->
-          FP s1 s2 l           : we can always shrink the freshness window (freshness_pre_shrink_upper_bound)
-
-     P3. FP s1 s2 l ->
-          incLocal s1 = (s2,r) ->
-          alist_fresh r l      : the whole point, the freshness window indeed generates fresh ids (freshness_pre_alist_fresh_specialized)
-
-     Q1. FQ s1 s2 l l          : if we don't extend the state, the postcondition is trivially true (freshness_pots_no_extension)
-
-     Q2. FQ s1 s2 l1 l2 ->
-         FQ s2 s3 l2 l3 ->
-         FQ s1 s3 l1 l3        : the postcondition is transitive (freshness_post_transitive)
-
-     Q3: incLocal s1 = (s2,r) ->
-         FQ s1 s2 l l[r->v]     : the postcondition is compatible with extension by generated variables (freshness_post_incLocal)
-
-     PQ. FP s1 s3 l1 ->
-         FQ s1 s2 l1 l2 ->
-         FP s2 s3 l2           : linking the pre and postcondition: if we have the precondition for a long computation,
-                                 and establish the postcondition at a mid point, we can recover the precondition at this point for the remaining of the computation.
-                                 (freshness_chain)
-
-   *)
-
-  (* If we have not extended the local state, certainly we did not extend it out the required bound *)
-  Lemma freshness_post_no_extension: forall s1 s2 l, freshness_post s1 s2 l l.
-  Proof.
-    intros; red; intros.
-    intuition.
-  Qed.
-
-  Lemma freshness_post_inclocal : forall s1 s2 l x v,
-      incLocal s1 ≡ inr (s2,x) ->
-      freshness_post s1 s2 l (alist_add x v l).
-  Proof.
-    intros * INC.
-    cbn in *.
-    apply lid_bound_between_incLocal in INC.
-    red; intros.
-    destruct (id ?[ Logic.eq ] x) eqn:EQ.
-    - rewrite rel_dec_correct in EQ; subst; auto.
-    - apply neg_rel_dec_correct in EQ.
-      apply In_add_In_ineq in H; auto.
-      intuition.
-  Qed.
-
-  (* Weakens the freshness precondition: if we know that the range [|s1;s3|] is fresh in [l],
-         we can always lower [s3].
-         This is useful to derive the precondition of the first inductive hypotheses when dealing with nary operators.
-   *)
-  Lemma freshness_pre_shrink_upper_bound :
-    forall s1 s2 s3 l,
-      freshness_pre s1 s3 l ->
-      s2 << s3 -> (* Also works with non-strict *)
-      freshness_pre s1 s2 l.
-  Proof.
-    (* intros; eapply new_state_invariant_shrink; eauto. *)
-  Admitted.
-
-  Lemma freshness_chain: forall s1 s2 s3 l1 l2 ,
-      freshness_pre s1 s3 l1 ->
-      freshness_post s1 s2 l1 l2 ->
-      freshness_pre s2 s3 l2.
-  Proof.
-  Admitted.
-
-  Lemma freshness_post_transitive :
-    forall s1 s2 s3 l1 l2 l3,
-      freshness_post s1 s2 l1 l2 ->
-      freshness_post s2 s3 l2 l3 ->
-      freshness_post s1 s3 l1 l3.
-  Admitted.
-
-  Lemma freshness_pre_alist_fresh_specialized:
-    forall s1 s2 l id,
-      freshness_pre s1 s2 l ->
-      incLocal s1 ≡ inr (s2,id) ->
-      alist_fresh id l.
-  Proof.
-    intros * ? INCL.
-    eapply freshness_pre_alist_fresh; eauto with irs_lt.
-  Qed.
-
-  Ltac forwardr H H' :=
-    match type of H with
-    | ?P -> _ => assert P as H'; [| specialize (H H')]
-    end.
-  Tactic Notation "forwardr" ident(H) ident(H') := forwardr H H'.
-  
-  Create HintDb fresh.
-  Hint Resolve freshness_post_no_extension: fresh.
-  Hint Resolve freshness_post_inclocal : fresh.
-
-  Definition lift_fresh (P: local_env -> Prop) : Rel_cfg := fun _ '(_,(l,_)) => P l.
-
-  Notation fresh_pre := (fun s1 s2 => lift_fresh (freshness_pre s1 s2)). 
-  Notation fresh_post := (fun s1 s2 l => lift_fresh (freshness_post s1 s2 l)). 
-  Ltac splits :=
-    repeat match goal with
-             | |- _ /\ _ => split
-             | |- (_ ⩕ _) _ _ => split
-           end.
-
-  Arguments freshness_pre : simpl never.
-  Arguments freshness_post : simpl never.
-  Arguments lift_fresh /.
-
-  Ltac solve_fresh :=
-    eauto with fresh;
-    match goal with
-    | h: freshness_pre ?s ?s' ?l |- freshness_pre ?s _ ?l => apply freshness_pre_shrink_upper_bound with (1 := h); solve_local_count
-    | h: freshness_pre _ ?s _ |- freshness_pre _ ?s _ => apply freshness_chain with (1 := h); solve_fresh
-    | h: freshness_post _ ?s _ ?x |- freshness_pre ?s _ ?x => eapply freshness_chain with (2 := h); solve_fresh
-    | |- freshness_post _ _ _ _ => first [eassumption | eapply freshness_post_inclocal; eassumption | eapply freshness_post_transitive; [eassumption |]]; solve_fresh
-    end.
-
-  Ltac solve_state_invariant :=
-    cbn;
-    match goal with
-      |- state_invariant _ _ _ (_, (alist_add _ _ _, _)) =>
-      eapply state_invariant_add_fresh; [now eauto | (eassumption || solve_state_invariant) | solve_fresh]
-    end.
-
   Lemma genNExpr_correct_ind :
     forall (* Compiler bits *) (s1 s2: IRState)
       (* Helix  bits *)   (nexp: NExpr) (σ: evalContext) (memH: memoryH) 
@@ -373,7 +166,20 @@ Require Import LidBound.
       specialize (IHnexp1 _ _ σ memH _ _ g l memV Heqs).
       forward IHnexp1.
       { split; auto.
+
+  match goal with
+  | h: freshness_pre ?s ?s' ?l |- freshness_pre ?s _ ?l => apply freshness_pre_shrink_up with (1 := h) end.  solve_local_count.
+  | h: freshness_pre _ ?s _ |- freshness_pre _ ?s _ => apply freshness_chain with (1 := h); solve_fresh
+  | h: freshness_post _ ?s _ ?x |- freshness_pre ?s _ ?x => eapply freshness_chain with (2 := h); solve_fresh
+  | |- freshness_post _ _ _ _ => first [eassumption | eapply freshness_post_inclocal; eassumption | eapply freshness_post_transitive; [eassumption |]]; solve_fresh
+  end.
+
+  
         solve_fresh.
+
+
+        unfold IRState_lt, IRState_le in *; get_local_count_hyps. lia.
+        solve_local_count_tac.
       }
       forward IHnexp1; eauto.
      
